theories/Lambda/ExprDsimpl.v
@@ -11,7 +11,7 @@ Require Import ExtLib.Tactics.
 Require Import MirrorCore.EnvI.
 Require Import MirrorCore.SymI.
 Require Import MirrorCore.ExprI.
-Require Import MirrorCore.Lambda.TypesI2.
+Require Import MirrorCore.TypesI.
 Require Import MirrorCore.Lambda.ExprCore.
 Require Import MirrorCore.Lambda.ExprDI.
 
@@ -21,136 +21,158 @@ Set Strict Implicit.
 Module ExprDenote <: ExprDenote.
 
   Section with_types.
+    Context {typ : Type}.
     Context {func : Type}.
-    Context {RType_typD : RType}.
+    Context {RType_typD : RType typ}.
     Context {Typ2_Fun : Typ2 _ Fun}.
-    Context {RSym_func : RSym typD func}.
+    Context {RSym_func : RSym func}.
 
     (** Reasoning principles **)
-    Context {RTypeOk_typD : @RTypeOk _}.
+    Context {RTypeOk_typD : RTypeOk}.
     Context {Typ2Ok_Fun : Typ2Ok Typ2_Fun}.
     Context {RSymOk_func : RSymOk RSym_func}.
 
-    Let typ_arr : typ -> typ -> typ := @typ2 _ _ _.
-    Let arr_match := @typ2_match _ _ _.
+    Let typ_arr : typ -> typ -> typ := @typ2 _ _ _ _.
+    Let arr_match := @typ2_match _ _ _ _.
     Let typD_arr
-    : forall ts a b, typD ts (typ_arr a b) = (typD ts a -> typD ts b)
-      := @typ2_cast _ _ _.
+    : forall a b, typD (typ_arr a b) = (typD a -> typD b)
+      := @typ2_cast _ _ _ _.
 
 
-    Global Instance RelDec_Rty ts : RelDec (Rty ts) :=
-    { rel_dec := fun a b => match type_cast ts a b with
+    Global Instance RelDec_Rty : RelDec Rty :=
+    { rel_dec := fun a b => match type_cast a b with
                               | Some _ => true
                               | None => false
                             end }.
 
-    Global Instance RelDec_Correct_Rty ts : @RelDec_Correct _ (Rty ts) _.
+    Global Instance RelDec_Correct_Rty : @RelDec_Correct _ Rty _.
     Proof.
       constructor. unfold rel_dec; simpl.
-      intros; consider (type_cast ts x y); intros.
+      intros; consider (type_cast x y); intros.
       split; auto. apply type_cast_total in H; eauto with typeclass_instances.
       intuition.
     Qed.
 
-    Definition Rcast T {ts a b} (pf : Rty ts a b) : T (typD ts a) -> T (typD ts b) :=
+    Definition Rcast T {a b} (pf : Rty a b) : T (typD a) -> T (typD b) :=
       Relim T (Rsym pf).
 
     Definition Rcast_val
-    : forall {ts a b} (pf : Rty ts a b), typD ts a -> typD ts b :=
+    : forall {a b} (pf : Rty a b), typD a -> typD b :=
       @Rcast (fun T => T).
 
+(*
     Definition OpenT ts := ResType.OpenT (typD ts).
     Definition Open_UseV := ResType.Open_UseV.
     Definition Open_UseU := ResType.Open_UseU.
-    Definition Open_Inj ts tus tvs := Eval simpl in @pure (OpenT ts tus tvs) _.
+*)
+    Instance Applicative_exprT tus tvs : Applicative (exprT tus tvs) :=
+    { pure := fun _ x _ _ => x
+    ; ap   := fun _ _ f g x y => (f x y) (g x y)
+    }.
 
-    Definition Open_App {ts tus tvs t u}
-    : OpenT ts tus tvs (typD ts (typ_arr t u)) -> OpenT ts tus tvs (typD ts t) -> OpenT ts tus tvs (typD ts u) :=
-      match eq_sym (typD_arr ts t u) in _ = T
-            return OpenT ts tus tvs T ->
-                   OpenT ts tus tvs (typD ts t) ->
-                   OpenT ts tus tvs (typD ts u)
+    Definition exprT_Inj tus tvs : forall T, T -> exprT tus tvs T :=
+      Eval simpl in @pure (@exprT typ RType_typD tus tvs) _.
+
+    Definition exprT_App {tus tvs t u}
+    : exprT tus tvs (typD (typ_arr t u)) -> exprT tus tvs (typD t) -> exprT tus tvs (typD u) :=
+      match eq_sym (typD_arr t u) in _ = T
+            return exprT tus tvs T ->
+                   exprT tus tvs (typD t) ->
+                   exprT tus tvs (typD u)
       with
         | eq_refl => fun f x => fun us vs => (f us vs) (x us vs)
       end.
 
     Section OpenT.
-      Variable ts : list Type.
-      Variables tus tvs : tenv typ.
+      Variable tus : tenv (ctyp typ).
+      Variable tvs : tenv typ.
 
       (** Auxiliary definitions **)
+(*
       Definition Open_GetUAs (n : nat) (t : typ) :
-        option (OpenT ts tus tvs (typD ts t)) :=
+        option (exprT tus tvs (typD t)) :=
         bind (m := option)
-             (nth_error_get_hlist_nth (typD ts) tus n)
+             (nth_error_get_hlist_nth ctxD tus n)
              (fun t_get =>
                 let '(existT t' get) := t_get in
                 bind (m := option)
-                     (type_cast ts t' t)
+                     (type_cast t' t)
                      (fun cast =>
                         ret (fun us vs => Rcast_val cast (get us)))).
+*)
 
       Definition Open_GetVAs (n : nat) (t : typ) :
-        option (OpenT ts tus tvs (typD ts t)) :=
+        option (exprT tus tvs (typD t)) :=
         bind (m := option)
-             (nth_error_get_hlist_nth (typD ts) tvs n)
+             (nth_error_get_hlist_nth (typD) tvs n)
              (fun t_get =>
                 let '(existT t' get) := t_get in
                 bind (m := option)
-                     (type_cast ts t' t)
+                     (type_cast t' t)
                      (fun cast =>
                         ret (fun us vs => Rcast_val cast (get vs)))).
 
     End OpenT.
 
-    Definition Open_Abs {ts tus tvs t u}
-    : OpenT ts tus (t :: tvs) (typD ts u) ->
-      OpenT ts tus tvs (typD ts (typ_arr t u)) :=
-      match eq_sym (typD_arr ts t u) in _ = T
-            return OpenT ts tus (t :: tvs) (typD ts u) -> OpenT ts tus tvs T
+    Definition Open_Abs {tus tvs t u}
+    : exprT tus (t :: tvs) (typD u) ->
+      exprT tus tvs (typD (typ_arr t u)) :=
+      match eq_sym (typD_arr t u) in _ = T
+            return exprT tus (t :: tvs) (typD u) -> exprT tus tvs T
       with
         | eq_refl => fun f => fun us vs x => f us (Hcons x vs)
       end.
 
-    Definition funcAs {ts} (f : func) (t : typ) : option (typD ts t) :=
+    Definition funcAs (f : func) (t : typ) : option (typD t) :=
       match typeof_sym f as Z
-            return Z = typeof_sym f -> option (typD ts t)
+            return Z = typeof_sym f -> option (typD t)
       with
         | None => fun _ => None
         | Some T => fun pf =>
-                      match type_cast ts T t with
+                      match type_cast T t with
                         | None => None
                         | Some cast =>
                           Rcast option cast
                                 (Some (match pf in _ = Z
                                              return match Z with
-                                                      | Some t => typD nil t
+                                                      | Some t => typD t
                                                       | None => unit
-                                                    end -> typD ts _
+                                                    end -> typD _
                                        with
-                                         | eq_refl => fun x => type_weaken ts _ x
+                                         | eq_refl => fun x => x
                                        end (symD f)))
                       end
       end eq_refl.
 
     Section typeof_expr.
-      Variable ts : list Type.
-      Variable tus : tenv typ.
+      Variable tus : tenv (ctyp typ).
 
       Definition type_of_apply (tv x : typ) : option typ :=
-        arr_match (fun _ => option typ) ts tv
+        arr_match (fun _ => option typ) tv
                   (fun d r =>
-                     match type_cast ts d x with
+                     match type_cast d x with
                        | Some _ => Some r
                        | None => None
                      end)
                   None.
 
-      Fixpoint typeof_expr (tvs : tenv typ) (e : expr typ func)
+      Require Import ExtLib.Structures.Traversable.
+      Require Import ExtLib.Data.List.
+
+      Fixpoint typeof_expr (tvs : tenv typ) (e : expr typ func) {struct e}
       : option typ :=
         match e with
         | Var x  => nth_error tvs x
-        | UVar x => nth_error tus x
+        | UVar x es =>
+          match nth_error tus x with
+            | None => None
+            | Some {| cctx := ctx ; vtyp := vtyp |} =>
+              match mapT_list _ _ (typeof_expr tvs) es with
+                | None => None
+                | Some ts =>
+                  if ts ?[ eq ] ctx then Some vtyp else None
+              end
+          end
         | Inj f => typeof_sym f
         | App e e' =>
           match typeof_expr tvs e
@@ -169,33 +191,51 @@ Module ExprDenote <: ExprDenote.
     End typeof_expr.
 
     Section exprD'.
-      Variable ts : list Type.
-      Variable tus : tenv typ.
+      Variable tus : tenv (ctyp typ).
+
+      Fixpoint applyEach tvs (rec : forall t, expr typ func -> option (exprT tus tvs (typD t)))
+               (ls : list typ) (es : list (expr typ func)) rT {struct es}
+      : option (ctxD {| cctx := ls ; vtyp := rT |} -> exprT tus tvs (typD rT)) :=
+        match ls as ls , es
+              return option (ctxD {| cctx := ls ; vtyp := rT |} -> exprT tus tvs (typD rT))
+        with
+          | nil , nil => Some (fun x _ _ => x Hnil)
+          | nil , _ :: _ => None
+          | _ :: _ , nil => None
+          | l :: ls , e :: es =>
+            match rec l e
+                , applyEach rec ls es rT
+            with
+              | None , _ => None
+              | Some _ , None => None
+              | Some eD , Some rD => Some (fun f us vs => rD (fun x => f (Hcons (eD us vs) x)) us vs)
+            end
+        end.
 
       Fixpoint exprD' (tvs : tenv typ) (t : typ) (e : expr typ func)
-      : option (OpenT ts tus tvs (typD ts t)) :=
-        match e return option (OpenT ts tus tvs (typD ts t)) with
-          | Var v => @Open_GetVAs ts tus tvs v t
+      : option (exprT tus tvs (typD t)) :=
+        match e return option (exprT tus tvs (typD t)) with
+          | Var v => @Open_GetVAs tus tvs v t
           | Inj f =>
             bind (m := option)
-                 (@funcAs _ f t)
+                 (@funcAs f t)
                  (fun val =>
-                    ret (@Open_Inj ts tus tvs _ val))
+                    ret (@exprT_Inj tus tvs _ val))
           | App f x =>
             bind (m := option)
-                 (typeof_expr ts tus tvs x)
+                 (typeof_expr tus tvs x)
                  (fun d =>
                     bind (m := option)
                          (exprD' tvs (typ_arr d t) f)
                          (fun f =>
                             bind (m := option)
                                  (exprD' tvs d x)
-                                 (fun x => ret (@Open_App ts _ _ _ _ f x))))
+                                 (fun x => ret (@exprT_App _ _ _ _ f x))))
           | Abs t' e =>
-            arr_match (fun T => option (OpenT ts tus tvs T)) ts t
+            arr_match (fun T => option (exprT tus tvs T)) t
                       (fun d r =>
                          bind (m := option)
-                              (type_cast ts d t')
+                              (type_cast d t')
                               (fun cast =>
                                  bind (m := option)
                                       (exprD' (t' :: tvs) r e)
@@ -203,43 +243,51 @@ Module ExprDenote <: ExprDenote.
                                          ret (fun us vs x =>
                                                 val us (Hcons (Rcast_val cast x) vs)))))
                       None
-          | UVar u => @Open_GetUAs ts tus tvs u t
+          | UVar u es => (* @Open_GetUAs ts tus tvs u t *)
+            bind (m := option)
+                 (OpenT.OpenT_Use ctxD tus  u)
+                 (fun ctx_val =>
+                    None
+
+)
         end.
     End exprD'.
 
     (** Equations **)
     Theorem exprD'_Var
-    : RTypeOk _ -> Typ2Ok Typ2_Fun -> RSymOk RSym_func ->
-      forall ts tus tvs t v,
-        exprD' ts tus tvs t (Var v) =
+    : RTypeOk -> Typ2Ok Typ2_Fun -> RSymOk RSym_func ->
+      forall tus tvs t v,
+        exprD' tus tvs t (Var v) =
         bind (m := option)
-             (nth_error_get_hlist_nth (typD ts) tvs v)
+             (nth_error_get_hlist_nth (typD) tvs v)
              (fun t_get =>
                 let '(existT t' get) := t_get in
                 bind (m := option)
-                     (type_cast ts t' t)
+                     (type_cast t' t)
                      (fun cast =>
                         ret (fun us vs => Rcast_val cast (get vs)))).
     Proof. reflexivity. Qed.
 
+(*
     Theorem exprD'_UVar
-    : RTypeOk _ -> Typ2Ok Typ2_Fun -> RSymOk RSym_func ->
-      forall ts tus tvs t u,
-        exprD' ts tus tvs t (UVar u) =
+    : RTypeOk -> Typ2Ok Typ2_Fun -> RSymOk RSym_func ->
+      forall tus tvs t u es,
+        exprD' tus tvs t (UVar u es) =
         bind (m := option)
-             (nth_error_get_hlist_nth (typD ts) tus u)
+             (nth_error_get_hlist_nth (typD) tus u)
              (fun t_get =>
                 let '(existT t' get) := t_get in
                 bind (m := option)
-                     (type_cast ts t' t)
+                     (type_cast t' t)
                      (fun cast =>
                         ret (fun us vs => Rcast_val cast (get us)))).
     Proof. reflexivity. Qed.
+*)
 
     Theorem exprD'_Inj
-    : RTypeOk _ -> Typ2Ok Typ2_Fun -> RSymOk RSym_func ->
-      forall ts tus tvs t s,
-        exprD' ts tus tvs t (Inj s) =
+    : RTypeOk -> Typ2Ok Typ2_Fun -> RSymOk RSym_func ->
+      forall tus tvs t s,
+        exprD' tus tvs t (Inj s) =
         bind (m := option)
              (funcAs s t)
              (fun val =>
@@ -247,30 +295,30 @@ Module ExprDenote <: ExprDenote.
     Proof. reflexivity. Qed.
 
     Lemma exprD'_App'
-    : forall ts tus tvs t f x,
-        exprD' ts tus tvs t (App f x) =
+    : forall tus tvs t f x,
+        exprD' tus tvs t (App f x) =
         bind (m := option)
-             (typeof_expr ts tus tvs x)
+             (typeof_expr tus tvs x)
              (fun d =>
                 bind (m := option)
-                     (exprD' ts tus tvs (typ_arr d t) f)
+                     (exprD' tus tvs (typ_arr d t) f)
                      (fun f =>
                         bind (m := option)
-                             (exprD' ts tus tvs d x)
-                             (fun x => ret (@Open_App ts _ _ _ _ f x)))).
+                             (exprD' tus tvs d x)
+                             (fun x => ret (@exprT_App _ _ _ _ f x)))).
     Proof. reflexivity. Qed.
 
     Theorem exprD'_Abs
-    : RTypeOk _ -> Typ2Ok Typ2_Fun -> RSymOk RSym_func ->
-      forall ts tus tvs t t' e,
-        exprD' ts tus tvs t (Abs t' e) =
-        arr_match (fun T => option (OpenT ts tus tvs T)) ts t
+    : RTypeOk -> Typ2Ok Typ2_Fun -> RSymOk RSym_func ->
+      forall tus tvs t t' e,
+        exprD' tus tvs t (Abs t' e) =
+        arr_match (fun T => option (exprT tus tvs T)) t
                   (fun d r =>
                      bind (m := option)
-                          (type_cast ts d t')
+                          (type_cast d t')
                           (fun cast =>
                              bind (m := option)
-                                  (exprD' ts tus (t' :: tvs) r e)
+                                  (exprD' tus (t' :: tvs) r e)
                                   (fun val =>
                                      ret (fun us vs x =>
                                             val us (Hcons (Rcast_val cast x) vs)))))
@@ -278,27 +326,27 @@ Module ExprDenote <: ExprDenote.
     Proof. reflexivity. Qed.
 
     Theorem exprD'_App
-    : RTypeOk _ -> Typ2Ok Typ2_Fun -> RSymOk RSym_func ->
-      forall ts tus tvs t f x,
-        exprD' ts tus tvs t (App f x) =
+    : RTypeOk -> Typ2Ok Typ2_Fun -> RSymOk RSym_func ->
+      forall tus tvs t f x,
+        exprD' tus tvs t (App f x) =
         bind (m := option)
-             (typeof_expr ts tus tvs x)
+             (typeof_expr tus tvs x)
              (fun t' =>
-                bind (exprD' ts tus tvs (typ_arr t' t) f)
+                bind (exprD' tus tvs (typ_arr t' t) f)
                      (fun f =>
-                        bind (exprD' ts tus tvs t' x)
+                        bind (exprD' tus tvs t' x)
                              (fun x =>
-                                ret (Open_App f x)))).
+                                ret (exprT_App f x)))).
     Proof. reflexivity. Qed.
 
     Theorem exprD'_respects
-    : RTypeOk _ -> Typ2Ok Typ2_Fun -> RSymOk RSym_func ->
-      forall ts tus tvs t t' e (pf : Rty ts t' t),
-        exprD' ts tus tvs t e =
-        Rcast (fun T => option (OpenT ts tus tvs T)) pf
-              (exprD' ts tus tvs t' e).
+    : RTypeOk -> Typ2Ok Typ2_Fun -> RSymOk RSym_func ->
+      forall tus tvs t t' e (pf : Rty t' t),
+        exprD' tus tvs t e =
+        Rcast (fun T => option (exprT tus tvs T)) pf
+              (exprD' tus tvs t' e).
     Proof.
-      destruct pf. change (eq_refl t') with (Rrefl ts t').
+      destruct pf. change (eq_refl t') with (Rrefl t').
       unfold Rcast. rewrite Relim_refl; eauto with typeclass_instances.
     Qed.
 
