theories/ExprProp.v
@@ -27,7 +27,7 @@ Section semantic.
     end.
 
   Definition Provable tus tvs (e : expr)
-  : option (OpenT tus tvs Prop) :=
+  : option (exprT tus tvs Prop) :=
     match exprD' tus tvs e tvProp with
       | None => None
       | Some p => Some (match @typ0_cast _ _ _ _  in _ = t
@@ -56,7 +56,7 @@ Section semantic.
   Qed.
 
   Definition AllProvable tus tvs (es : list expr)
-  : option (OpenT tus tvs Prop) :=
+  : option (exprT tus tvs Prop) :=
     match mapT (T:=list) (F:=option) (Provable tus tvs) es with
       | None => None
       | Some Ps => Some (fun us vs => Forall (fun x => x us vs) Ps)
