theories/InstantiateI.v
@@ -31,19 +31,19 @@ Section definitions.
   (** instantiate **)
   Variable instantiate : (nat -> list expr -> option expr) -> nat -> expr -> expr.
 
-  Definition sem_preserves_if (tus : tenv (tenv typ * typ)) (tvs : tenv typ)
-             (P : OpenT tus tvs Prop)
+  Definition sem_preserves_if (tus : tenv (ctyp typ)) (tvs : tenv typ)
+             (P : exprT tus tvs Prop)
              (f : nat -> list expr -> option expr) : Prop :=
     forall u e es t get vals,
       f u es = Some e ->
       nth_error_get_hlist_nth _ tus u = Some (@existT _ _ t get) ->
-      hlist_build (fun T => OpenT tus tvs (typD T))
-                  (fun t e => exprD' tus tvs e t) (fst t) es = Some vals ->
+      hlist_build (fun T => exprT tus tvs (typD T))
+                  (fun t e => exprD' tus tvs e t) t.(cctx) es = Some vals ->
       exists eD,
-        exprD' tus tvs e (snd t) = Some eD /\
+        exprD' tus tvs e t.(vtyp) = Some eD /\
         forall us vs,
           P us vs ->
-          get us (hlist_map (fun t (x : OpenT tus tvs (typD t)) => x us vs) vals) = eD us vs.
+          get us (hlist_map (fun t (x : exprT tus tvs (typD t)) => x us vs) vals) = eD us vs.
 
   (** TODO **)
 (*
